dimsum_examples/iris/my_echo.v
@@ -1,62 +1,5 @@
 From iris.proofmode Require Import proofmode.
 From iris.bi.lib Require Import fixpoint.
-
-(* NOTE - BI the logic of "bunched implications" *)
-Section bi_loop.
-  Context {PROP : bi} {A : Type} (body : (A → PROP) → (A → PROP)).
-
-  Definition bi_loop_pre (bi_loop : leibnizO A -d> PROP) :
-    leibnizO A -d> PROP := λ a,
-    (∀ Φ, □ (∀ x, bi_loop x -∗ Φ x) -∗ body Φ a)%I.
-
-  Global Instance bi_loop_pre_ne n:
-    Proper ((dist n ==> dist n) ==> dist n ==> dist n) bi_loop_pre.
-  Proof.
-    move => ?? Hsim ?? ->. rewrite /bi_loop_pre.
-    repeat (f_equiv || eapply Hsim || reflexivity).
-  Qed.
-
-  Lemma bi_loop_pre_mono loop1 loop2:
-    ⊢ □ (∀ a, loop1 a -∗ loop2 a)
-    → ∀ a , bi_loop_pre loop1 a -∗ bi_loop_pre loop2 a.
-  Proof.
-    iIntros "#Hinner" (a) "Hsim". iIntros (?) "#HC".
-    iApply "Hsim". iIntros "!>" (?) "?". iApply "HC". by iApply "Hinner".
-  Qed.
-
-  Local Instance bi_loop_pre_monotone :
-    BiMonoPred bi_loop_pre.
-  Proof.
-    constructor.
-    - iIntros (Π Ψ ??) "#Hinner". iIntros (?) "Hsim" => /=. iApply bi_loop_pre_mono; [|done].
-      iIntros "!>" (?) "HΠ". by iApply ("Hinner" $! _).
-    - move => bi_loop Hsim n a1 a2 /= ?.
-      apply bi_loop_pre_ne; eauto. move => ??? /=. by apply: Hsim.
-  Qed.
-End bi_loop.
-
-Definition bi_loop {PROP : bi} {A} (body : (A → PROP) → (A → PROP)) (a : A) :=
-  bi_greatest_fixpoint (bi_loop_pre body) a.
-
-Section bi_loop.
-  Context {PROP : bi} {A : Type} (body : (A → PROP) → (A → PROP)).
-
-  Local Existing Instance bi_loop_pre_monotone.
-  Lemma bi_loop_eq a:
-    bi_loop body a ⊣⊢ bi_loop_pre body (bi_loop body) a.
-  Proof. rewrite /bi_loop.
-         apply: greatest_fixpoint_unfold.
-  Qed.
-
-  Lemma bi_loop_step a:
-    (∀ Φ, □ (∀ a, bi_loop body a -∗ Φ a) -∗ body Φ a) ⊢ bi_loop body a.
-  Proof. by rewrite bi_loop_eq. Qed.
-
-  Lemma bi_loop_unfold a:
-    bi_loop body a ⊢ body (bi_loop body) a.
-  Proof. rewrite bi_loop_eq. iIntros "Hl". iApply "Hl". iIntros "!>" (?) "$". Qed.
-End bi_loop.
-
 From dimsum.examples.iris Require Import asm rec2.
 Set Default Proof Using "Type".
 
@@ -65,20 +8,13 @@ Local Open Scope Z_scope.
 (* TODO: upstream? *)
 Arguments subst_static _ !_ /.
 
-Local Ltac go :=
-  clear_spec.
-Local Ltac go_s :=
-  tstep_s; go.
-Local Ltac go_i :=
-  tstep_i; go.
-
 Definition echo_rec : fndef := {|
   fd_args := [];
   fd_static_vars := [];
   fd_vars := [];
   fd_body := LetE "c" (rec.Call (Val (ValFn "getc")) []) $
              LetE "_" (rec.Call (Val (ValFn "putc")) [Var "c"]) $
-             rec.Call (Val (ValFn "echo")) [];
+             Val (ValNum 0);
   fd_static := I
 |}.
 
@@ -96,439 +32,14 @@ Definition TCallRet {S} (f : string) (vs : list val) (h : heap_state) :
   else
     TUb.
 
-(* NOTE: Trying to formulate some things for TCallRet *)
-Section TCallRet.
-
-Context `{!dimsumGS Σ} `{!specGS} {S : Type}.
-(* Canonical Structure spec_mod_lang. *)
-
-(* NOTE - In src position we only need to ensure `Outgoing Call` and any incoming event *)
-(* This cannot be quite true, in case it's not undefined, I'll have to refine it ? *)
-
-(* The statement holds, assuming the following restriction on Π.
-   ...
- *)
-(* TODO: What does it mean if POST is unused in the hypothesis *)
-
-Compute m_state (spec_trans (io_type * rec_ev) S).
-(* Provable spec, but actually not what I'd want. I am now requiring a Return rather than case splitting on it *)
-Lemma sim_src_TCallRet f vs h (k: _ → spec rec_event S void) Π Φ :
-  switch Π ({{κ σ POST,
-    ∃ f' vs' h1,
-      ⌜f' = f⌝ ∗ ⌜vs' = vs⌝ ∗ ⌜h1 = h⌝ ∗
-      ⌜κ = Some (Outgoing, ERCall f vs h)⌝ ∗
-      POST Src _ (spec_trans rec_event S) ({{σ' Π',
-        ⌜σ = σ'⌝ ∗ ∃ v h',
-        switch Π' ({{κ σ POST,
-            ⌜κ = Some (Incoming, ERReturn v h')⌝ ∗
-          POST Src _ (spec_trans rec_event S) ({{ σ'' Π'',
-            ⌜σ = σ''⌝ ∗
-            ⌜Π = Π''⌝ ∗
-            SRC (k (v, h')) @ Π {{ Φ }}
-            }})
-        }})
-        }})
-    }}) -∗
-  SRC (Spec.bind (TCallRet f vs h) k) @ Π {{ Φ }}.
-Proof.
-  iIntros "HC" => /=. rewrite /TCallRet bind_bind.
-  iApply sim_gen_TVis. iIntros (s) "Hs". iIntros "% % /=". iIntros "[% [% HΠ]]". subst.
-  iApply "HC" => /=. iSplit!.
-  iIntros (??) "[% [% [% HC]]]" => /=. subst.
-  iApply (sim_gen_expr_intro _ tt with "[Hs] [-]"); simpl; [done..|].
-  rewrite bind_bind.  iApply sim_src_TExist.
-  rewrite bind_bind. iApply sim_gen_TVis. iIntros (s') "Hs". iIntros (??) "[% [% HΠ']]" => /=.
-  unfold sim_gen_mapsto_state.
-  subst. iApply "HC" => /=. iSplit!.
-  iIntros (??) "[% [% H']]". subst.
-  iApply "HΠ". iSplit!. iSplitL "Hs". 1: done.
-  by rewrite bind_ret_l.
-  Qed.
-
-(* Lemma sim_src_TCallRet' f vs h (k: _ → spec rec_event S void) Π Φ : *)
-(*   switch Π ({{κ σ POST, *)
-(*     ∃ f' vs' h1, *)
-(*       ⌜f' = f⌝ ∗ ⌜vs' = vs⌝ ∗ ⌜h1 = h⌝ ∗ *)
-(*       ⌜κ = Some (Outgoing, ERCall f vs h)⌝ ∗ *)
-(*       POST Src _ (spec_trans rec_event S) ({{σ' Π', *)
-(*         ⌜σ = σ'⌝ ∗ ∃ v h' e, *)
-(*         switch Π' ({{κ σ POST, *)
-(*           ⌜κ = Some e⌝ ∗ *)
-(*           (* TODO: Obligation? *) *)
-(*           POST Src _ (spec_trans rec_event S) ({{ σ'' Π'', *)
-(*             ⌜κ = Some (Incoming, ERReturn v h')⌝ ∗ *)
-(*             ⌜σ = σ''⌝ ∗ *)
-(*             ⌜Π = Π''⌝ ∗ *)
-(*             SRC (k (v, h')) @ Π {{ Φ }} *)
-(*             }}) *)
-(*         }}) *)
-(*         }}) *)
-(*     }}) -∗ *)
-(*   SRC (Spec.bind (TCallRet f vs h) k) @ Π {{ Φ }}. *)
-(* Proof. *)
-(*   iIntros "HC" => /=. rewrite /TCallRet bind_bind. *)
-(*   iApply sim_gen_TVis. iIntros (s) "Hs". iIntros "% % /=". iIntros "[% [% HΠ]]". subst. *)
-(*   iApply "HC" => /=. iSplit!. *)
-(*   iIntros (??) "[% [% [% HC]]]" => /=. subst. *)
-(*   iApply (sim_gen_expr_intro _ tt with "[Hs] [-]"); simpl; [done..|]. *)
-(*   rewrite bind_bind.  iApply sim_src_TExist. *)
-(*   rewrite bind_bind. iApply sim_gen_TVis. iIntros (s') "Hs". iIntros (??) "[% [% HΠ']]" => /=. *)
-(*   subst. iApply "HC" => /=. iSplit!. *)
-(*   iIntros (??) "[% [% [% H']]]". simplify_eq. rewrite H0. *)
-(*   iApply "HΠ". iSplit!. iSplitL "Hs". 1: done. *)
-(*   by rewrite bind_ret_l. *)
-(*   Qed. *)
-
-End TCallRet.
-
-Definition echo_spec_body : spec rec_event unit unit :=
-  h ← TExist _;
-  '(c, h') ← TCallRet "getc" [] h;
-  TAssume (h = h');;
-  h ← TExist _;
-  '(_, h') ← TCallRet "putc" [c] h;
-  TAssume (h = h');;
-  TRet tt.
-
-Definition echo_spec : spec rec_event unit void :=
-  '(f, vs, h) ← TReceive (λ '(f, vs, h), (Incoming, ERCall f vs h));
-  TAssume (f = "echo");;
-  TAssume (vs = []);;
-  Spec.forever echo_spec_body.
-
-Lemma echo_refines_echo_spec_direct :
-  trefines (rec_mod echo_prog) (spec_mod echo_spec tt).
-Proof.
-  apply: tsim_implies_trefines => n0 /=.
-  (* Handle the initial call from the environment *)
-  tstep_i.
-  split! => ???? H.
-  tstep_s. eexists (_, _, _). go.
-  tstep_s. split!. go.
-  tstep_s => ?. go.
-  tstep_s => ?. go. destruct!.
-  (* Now prove the body by induction *)
-  unshelve eapply tsim_remember. { simpl. exact (λ _ '(Rec e _ f) '(t, _),
-    (* TODO: How does Michael think about this, I guess typically I would phrase an induction hypothesis
-      using an arbitrary kontext here *)
-    exists K,
-    t ≡ Spec.forever echo_spec_body ∧
-    e = expr_fill K ((Call (Val (ValFn "echo"))) (Val <$> [])) ∧
-    f = echo_prog). }
-  { eexists [ReturnExtCtx false]. split!. } { done. }
-  move => n _ Hloop [???] [??] [ctx[?[??]]] /=. destruct!/=.
-  go_s.
-  tstep_s. eexists. go.         (* NOTE: Introducing Heap *)
-  tstep_i. split!.
-  move => ??. destruct!/=.
-  rewrite /echo_prog in H. simplify_map_eq. split!.
-  (* NOTE: Start of getc *)
-  tstep_i => ?? [??]. simplify_eq. split!.
-  tstep_i. split!. move => ?.              (* NOTE - split between internal and external call *)
-  (* NOTE: Here we now have `Waiting true` *)
-  tstep_s. split!. go.
-  tstep_i.
-  split.
-  { (* NOTE: Here I now am getting a call back from the external call, i.e., because of TCallRet immediate UB *)
-    move => ?????.
-    tstep_s. eexists. go.
-    tstep_s. split!. go.
-    by tstep_s. }
-  move => ???.
-  tstep_s. eexists. go.
-  tstep_s. split!. go.
-  tstep_s => ?. go.
-  (* NOTE: Start of putc *)
-  tstep_s. eexists. go.
-  tstep_i. tstep_i. split!. move => ?.
-  tstep_s. split!. go.
-  tstep_i. split!.
-  { (* NOTE: Here I now am getting a call back from the external call, i.e., because of TCallRet immediate UB *)
-    move => ?????.
-    tstep_s. eexists. go.
-    tstep_s. split!. go.
-    by tstep_s. }
-  move => ???.
-  tstep_s. eexists. go.
-  tstep_s. split!. go.
-  tstep_s => ?.
-  rewrite bind_ret_l.
-  go. simplify_eq.
-  tstep_i.
-  eapply Hloop. { done. }
-  eexists ([FreeACtx []] ++ ctx).
-  split!.
-Qed.
-
-Section echo.
-  Context `{!dimsumGS Σ} `{!recGS Σ}.
-
-  Lemma sim_echo' Π :
-    "echo" ↪ Some echo_rec -∗
-    rec_fn_spec_hoare Tgt Π "echo" ({{ es POST0, ⌜es = []⌝ ∗
-      bi_loop ({{ LOOP _,
-        rec_fn_spec_hoare Tgt Π "getc" ({{ es POST,
-          ⌜es = []⌝ ∗
-        POST ({{ c,
-        rec_fn_spec_hoare Tgt Π "putc" ({{ es POST,
-          ⌜es = [Val c]⌝ ∗
-        POST ({{ _,
-          LOOP tt
-        }})}})}})}})}}) tt}}).
-  Proof. Admitted. (* I did this in the old echo file *)
-
-  Lemma sim_echo_spec Π γσ_s (σ : m_state (spec_trans _ unit)) :
-    "echo" ↪ Some echo_rec -∗
-    "getc" ↪ None -∗
-    "putc" ↪ None -∗
-    γσ_s ⤳ σ -∗
-    ⌜σ.1 ≡ Spec.forever echo_spec_body⌝ -∗
-    □ switch_external Π ({{ _ σ POST,
-        ∃ σ_s, γσ_s ⤳ σ_s ∗
-      POST (spec_trans _ unit) σ_s ({{ _ Π',
-      switch Π' ({{ κ σ_s' POST,
-       ⌜κ = None⌝ ∗
-      POST Tgt _ _ ({{ σ' Π', ⌜σ' = σ⌝ ∗ ⌜Π' = Π⌝ ∗ γσ_s ⤳ σ_s'}})}})}})}}) -∗
-    rec_fn_spec_hoare Tgt Π "echo" ({{ es _, ⌜es = []⌝}}).
-  Proof. Admitted.
-End echo.
-
-(* ********************************************************************************************** *)
-(* getc rec program that calls read *)
-(* ********************************************************************************************** *)
-
-Definition getc_rec : fndef := {|
-  fd_args := [];
-  fd_static_vars := [];
-  fd_vars := [("l", 1)];
-  fd_body := LetE "c" (rec.Call (Val (ValFn "read")) [Var "l"; Val 1]) $
-             Load (Var "l");
-  fd_static := I
-|}.
-Definition getc_prog : gmap string fndef :=
-  <["getc" := getc_rec]> $ ∅.
-
-Section getc.
-  Context `{!dimsumGS Σ} `{!recGS Σ}.
-  (* TODO: Does it make sense to think about it this way
-    { args = [] * ({ ∃ l v, ⌜es = [Val $ ValLoc l; Val $ 1]⌝ ∗ l ↦ v } read { ∃ c, l ↦ c}) } getc { ~res~ = c } *)
-
-  Lemma sim_getc Π :
-    "getc" ↪ Some getc_rec -∗
-    rec_fn_spec_hoare Tgt Π "getc" ({{ es POST0, ⌜es = []⌝ ∗
-      rec_fn_spec_hoare Tgt Π "read" ({{ es POST,
-        ∃ l v, ⌜es = [Val $ ValLoc l; Val $ 1]⌝ ∗ l ↦ v ∗
-      POST ({{ _,
-        ∃ c, l ↦ (ValNum c) ∗ POST0 ({{ vr, ⌜vr = ValNum c⌝}})}})}})}}).
-  Proof.
-    iIntros "#?".
-    iIntros (es Φ). iDestruct 1 as (->) "HΦ".
-    iApply sim_tgt_rec_Call_internal. 2: { done. } { done. }
-    iModIntro => /=.
-    iApply sim_tgt_rec_AllocA; [by econs|] => /=. iIntros (?) "Hl".
-    destruct ls as [|? []] => //=. 2: iDestruct!. iModIntro.
-    rewrite offset_loc_0. iDestruct "Hl" as "[[Hl _] _]".
-    iApply (sim_gen_expr_bind _ [LetECtx _ _] with "[-]") => /=.
-    iApply "HΦ". iSplit!. iFrame. iIntros (?) "[% [Hl HΦ]]".
-    iApply sim_tgt_rec_LetE. iIntros "!>" => /=.
-    iApply (sim_tgt_rec_Load with "Hl"). iIntros "Hl !>" => /=. iSplit!.
-    iFrame. by iApply "HΦ".
-  Qed.
-
-End getc.
-
-(* ********************************************************************************************** *)
-(* read rec program that reads `c` ints into the pointer `l` from a buffer of increasing numbers *)
-(* ********************************************************************************************** *)
-
-Definition read_mem_rec : fndef := {|
-  fd_args := ["l"; "c"];
-  fd_static_vars := [("pos", 1)];
-  fd_vars := [];
-  fd_body :=
-(*
-global pos = 0;
-read (l, c) {
-  if (c <= 0) {
-    return 0;
-  } else {
-    l <- pos;
-    pos <- *pos + 1;
-    ret = read(l + 1, c + (-1));
-    return ret + 1;
-  }
-}
-*)
-    If (BinOp (Var "c") LeOp (Val 0))
-      (Val 0)
-      (* NOTE: There is no sequencing *)
-      (LetE "_" (Store (Var "l") (Load (Var "pos"))) $
-       LetE "_" (Store (Var "pos") (BinOp (Load (Var "pos")) AddOp (Val 1))) $
-       LetE "ret" (rec.Call (Val (ValFn "read")) [
-                       BinOp (Var "l") OffsetOp (Val 1);
-                       BinOp (Var "c") AddOp (Val (-1))]) $
-       (BinOp (Var "ret") AddOp (Val 1)));
-  fd_static := I
-|}.
-Definition read_mem_prog : gmap string fndef :=
-  <["read" := read_mem_rec]> $ ∅.
-
-Section read_mem.
-  Context `{!dimsumGS Σ} `{!recGS Σ}.
-
-  Lemma sim_read_mem Π (lpos : loc) :
-    (* Given a static/global variable *)
-    lpos = (ProvStatic "read" 0, 0) →
-    (* "read" points to the function (internal) *)
-    "read" ↪ Some read_mem_rec -∗
-    rec_fn_spec_hoare Tgt Π "read" ({{ es POST0, ∃ l vs (pos : Z),
-      (* Arguments are a location and length of a list *)
-      ⌜es = [Val (ValLoc l); Val (length vs)]⌝ ∗
-      (* We own the global pointer *)
-      lpos ↦ pos ∗
-      (* We own the array [vs[0], vs[1], ... , vs[vs.length - 1]] *)
-      ([∗ map] l↦v∈array l vs, l ↦ v) ∗
-      POST0 ({{ vret,
-        (* We return the length of the list *)
-        ⌜vret = ValNum (length vs)⌝ ∗
-        (* The global pointer has been increased by length of the list *)
-        lpos ↦ (pos + length vs) ∗
-        (* We own the array [pos + 0, pos +1, ..., pos + (vs.length - 1)] *)
-        ([∗ map] l↦v∈array l (ValNum <$> seqZ pos (length vs)), l ↦ v)
-      }})}}).
-  Proof.
-    iIntros "%Hlpos #?". iApply rec_fn_spec_hoare_ctx. iIntros "#?".
-    iApply ord_loeb. { iAssumption. } iModIntro.
-    iIntros "#IH %es %Φ HΦ/=".
-    iDestruct "HΦ" as (? ? count) "[? [Hlpos [Hl H]]]".
-    (* Base Case *)
-    iDestruct!.
-    iApply sim_tgt_rec_Call_internal. 2: { done. } { done. }
-    (* FIXME: Maybe I can use this to try fiddling with auto indentation *)
-    iModIntro.
-    iApply sim_tgt_rec_AllocA; [done|]. iIntros (lcl) "Hlcl /=".
-    iModIntro.
-    (* NOTE: Bind the BinOp *)
-    iApply (sim_gen_expr_bind _ [IfCtx _ _]).
-    iApply sim_tgt_rec_BinOp. { reflexivity. } iModIntro.
-    iApply sim_tgt_rec_If. iModIntro.
-    (* Split into base and recursive case *)
-    destruct vs; simpl.
-    - iApply sim_gen_expr_stop.
-      iExists 0.
-      iSplit; [done|].
-      iSplitL "Hlcl".
-      { by destruct lcl. }
-      iApply "H". rewrite Z.add_0_r.
-      iSplit!.
-    - (* STORE 1 *)
-      iApply (sim_gen_expr_bind _ [LetECtx _ _]).
-      iApply (sim_gen_expr_bind _ [StoreRCtx _]).
-      iApply (sim_tgt_rec_Load with "Hlpos"). iIntros "Hlpos". iModIntro => /=.
-      (* NOTE: I need to unroll the separating conjunction and pass ownership of the first location *)
-      (* FIXME Why can't I use iRewrite *)
-      (* rewrite array_cons. iRewrite big_sepM_insert  in "Hl". *)
-      rewrite array_cons big_sepM_insert. 2 : { rewrite array_lookup_None. naive_solver lia. }
-      iDestruct "Hl" as "[Hl Hl']".
-      iApply (sim_tgt_rec_Store with "Hl"). iIntros. iModIntro.
-      iApply sim_tgt_rec_LetE. iModIntro. simpl.
-      (* STORE 2 *)
-      iApply (sim_gen_expr_bind _ [LetECtx _ _]).
-      iApply (sim_gen_expr_bind _ [StoreRCtx _]).
-      iApply (sim_gen_expr_bind _ [BinOpLCtx _ _]).
-      iApply (sim_tgt_rec_Load with "Hlpos"). iIntros "Hlpos !> /=".
-      iApply sim_tgt_rec_BinOp. { reflexivity. } iModIntro.
-      iApply (sim_tgt_rec_Store with "Hlpos"). iIntros "Hlpos !>".
-      iApply sim_tgt_rec_LetE. iModIntro. simpl.
-      (* Call + RETURN *)
-      iApply (sim_gen_expr_bind _ [LetECtx _ _]).
-      (* Handle arguments *)
-      iApply (sim_gen_expr_bind _ [CallCtx _ [] _]) => /=.
-      iApply sim_tgt_rec_BinOp. { reflexivity. } iModIntro.
-      iApply (sim_gen_expr_bind _ [CallCtx _ [_] _]).
-      iApply sim_tgt_rec_BinOp => /=.
-      (* FIXME: Why is this so hard :/ *)
-      { instantiate (1 := length vs). f_equal. rewrite Nat2Z.inj_succ.
-        change (_ + -1) with (Z.pred (Z.succ (length vs))). rewrite Z.pred_succ. reflexivity. } iModIntro.
-      (* Induction *)
-      iApply "IH". simpl.
-      (* TODO: That's a little awkward *)
-      do 3 iExists (_).
-      iSplit. { done. }
-      iSplitL "Hlpos". iAssumption.
-      iSplitL "Hl'". iAssumption.
-      iIntros (v') "[-> [Hlpos ?]]".
-      iApply sim_tgt_rec_LetE => /=. iModIntro.
-      iApply (sim_tgt_rec_BinOp). { reflexivity. } iModIntro.
-      iExists (_).
-      iSplit. done.
-      iSplitL "Hlcl". {by destruct lcl. }
-      iApply "H".
-      rewrite! Nat2Z.inj_succ.
-      iSplit. { done. }
-      iSplitL "Hlpos". { rewrite <-Z.add_assoc, Z.add_1_l. iApply "Hlpos". }
-      (* TODO: Rewrite at doesn't work *)
-      (* rewrite seqZ_cons at 2. *)
-      rewrite (seqZ_cons _ (Z.succ _)) => /=. 2 : { lia. }
-      rewrite array_cons.
-      (* FIXME: Why does iRewrite not work? *)
-      rewrite big_sepM_insert Z.pred_succ -Z.add_1_r. 2: { rewrite array_lookup_None. naive_solver lia. }
-      iFrame.
-  Qed.
-
-End read_mem.
-
 (* ********************************************************************************************** *)
 (* combined rec program that will return increasing numbers with each call *)
 (* ********************************************************************************************** *)
-
-Definition combined_prog : gmap string fndef :=
-  <["read" := read_mem_rec]> $ <["getc" := getc_rec]> $ ∅.
-
-Section combined.
+Section sim_getc.
   Context `{!dimsumGS Σ} `{!recGS Σ}.
 
-  Lemma sim_combined Π (lpos : loc) :
-    (* Given a static/global variable which holds the buffer (index into) *)
-    lpos = (ProvStatic "read" 0, 0) →
-    (* "read" points to the function we defined (internal) *)
-    "read" ↪ Some read_mem_rec -∗
-    "getc" ↪ Some getc_rec -∗
-    rec_fn_spec_hoare Tgt Π "getc" ({{ es POST, ∃ (pos : Z),
-      ⌜es = []⌝ ∗
-      lpos ↦ pos ∗
-      POST ({{ vr, ⌜vr = ValNum pos⌝ ∗ lpos ↦ (pos + 1)}})}}).
-  Proof.
-    iIntros "%Hlpos #Hread #Hgetc %args %Φ Hpre".
-    iApply sim_getc => /=; [done|].
-    iDestruct "Hpre" as "[%count [?[? HΦ]]]". iFrame.
-    rewrite /rec_fn_spec_hoare /rec_fn_spec.
-    iIntros "%args' %Φ' [%l [%v [Hargs' [Hl HΦ']]]]".
-    iApply sim_read_mem => /=. 1-2: done.
-    do 3 iExists (_). iFrame.
-    iSplitL "Hargs'". { instantiate (1 := [v]). iExact "Hargs'". }
-    iSplitL "Hl".
-    { rewrite /array => /=.
-      rewrite insert_empty kmap_singleton offset_loc_0 big_sepM_singleton. iAssumption. }
-    iIntros (v') "[? [? Hl]]" => /=.
-    iApply "HΦ'". iExists (_).
-    iSplitL "Hl".
-    { rewrite Z.add_0_l /array  => /=.
-      rewrite insert_empty kmap_singleton offset_loc_0 big_sepM_singleton. iAssumption. }
-    iIntros (v'') "?".
-    iApply "HΦ". iFrame.
-  Qed.
-
-End combined.
-
-(* ********************************************************************************************** *)
-(* combined rec program that will return increasing numbers with each call *)
-(* ********************************************************************************************** *)
-Section sim_spec.
-  Context `{!dimsumGS Σ} `{!recGS Σ}.
-
-  Definition getc_spec_priv : spec rec_event Z unit :=
-    (* Spec.forever( *)
+  Definition getc_spec: spec rec_event Z void :=
+    Spec.forever(
     (* Incoming call of getc *)
     '(f, vs, h) ← TReceive (λ '(f, vs, h), (Incoming, ERCall f vs h));
     TAssume (f = "getc");;
@@ -537,7 +48,7 @@ Section sim_spec.
     v ← TGet;
     TPut (v + 1);;
     (* Return old position *)
-    TVis (Outgoing, ERReturn (ValNum v) h).
+    TVis (Outgoing, ERReturn (ValNum v) h)).
 
   Lemma mstate_var_agree {S : TypeState} `{!mstateG Σ} γ (σ1 σ2 : S) :
     γ ⤳ σ1 -∗ γ ⤳ σ2 -∗ ⌜σ1 = σ2⌝.
@@ -546,115 +57,114 @@ Section sim_spec.
     inv H0. by dimsum.core.axioms.simplify_K.
   Qed.
 
-  (* REVIEW: Do I get all my states back? *)
-  Lemma sim_getc_spec_heap_priv `{!specGS} Π Φ k :
+  (* TODO: I am not using this Lemma anywhere *)
+  Lemma sim_getc_spec `{!specGS} Π Φ :
+    switch Π ({{ κ σ1 POST,
+      ∃ f es h, ⌜κ = Some (Incoming, ERCall f es h)⌝ ∗
+    POST Tgt _ _ ({{ σ' Π',
+      ∃ v, ⌜f = "getc"⌝ ∗ ⌜es = []⌝ ∗ spec_state v ∗ ⌜σ' = σ1⌝ ∗
+      ⌜Π' = Π⌝ ∗ (* I think this need not be true? - Check what it looks like - what's the difference between this and just requiring Π for the next switch *)
     switch Π ({{ κ σ POST,
-      ∃ f vs h, ⌜κ = Some (Incoming, ERCall f vs h)⌝ ∗
-      POST Tgt _ (spec_trans _ Z) ({{ σ' Π',
-        ∃ v, ⌜σ' = σ⌝ ∗ ⌜f = "getc"⌝ ∗ ⌜vs = []⌝ ∗ (spec_state v) ∗
-      switch Π' ({{ κ σ POST,
-      ⌜κ = (Some (Outgoing, ERReturn (ValNum v) h))⌝ ∗
-      spec_state (v + 1) ∗
-      POST Tgt _ (spec_trans _ Z) ({{σ'' Π'',
-        ⌜Π'' = Π⌝ ∗
-        ⌜σ'' = σ⌝ ∗
-        TGT k tt @ Π {{ Φ }}
-        }})
-      }})}})}}) -∗
-    TGT Spec.bind getc_spec_priv k @ Π {{ Φ }}.
+      ⌜κ = Some (Outgoing, ERReturn (ValNum v) h)⌝ ∗ spec_state (v + 1)
+    (* POST Tgt _ _ ({{ σ' Π', *)
+    (*   ⌜σ' = σ⌝ ∗ ⌜Π' = Π⌝ ∗ spec_state (v + 1) }})*)
+    }})}})}}) -∗
+    TGT getc_spec @ Π {{ Φ }}.
   Proof.
-    iDestruct 1 as "HC".
-    rewrite /TReceive bind_bind bind_bind.
+    iIntros "Hs".
+    rewrite /getc_spec unfold_forever /TReceive bind_bind -/getc_spec bind_bind.
     iApply (sim_tgt_TExist with "[-]"). iIntros ([[??]?]) "!>".
     rewrite bind_bind. setoid_rewrite bind_ret_l.
     iApply (sim_gen_TVis with "[-]").
-    iIntros (v) "Hs !>". simpl.
-    iIntros (??) "[% [% HΠ]]". simpl.
+    iIntros (v') "Hs' !>".
+    iIntros (??) "[% [% HΠ]]".
     subst.
-    iApply "HC". simpl. iSplit!. iIntros (??).
-    iDestruct 1 as (????) "[Hs' HC]". subst.
-    iApply (sim_gen_expr_intro _ tt with "[Hs]"); simpl; [done..|].
-    rewrite bind_bind. iApply (sim_tgt_TAssume with "[-]"); [done|]. iIntros "!>".
-    rewrite bind_bind. iApply (sim_tgt_TAssume with "[-]"); [done|]. iIntros "!>".
-    rewrite bind_bind. iApply (sim_gen_TGet with "[-]").
+    iApply "Hs" => /=. iSplit!. iIntros (??) => /=.
+    iDestruct 1 as (???) "[Hs [% [% HC]]]". subst.
+    iApply (sim_gen_expr_intro _ tt with "[Hs']"); simpl; [done..|]. rewrite bind_bind.
+    iApply (sim_tgt_TAssume with "[-]"); [done|]. iIntros "!>". rewrite bind_bind.
+    iApply (sim_tgt_TAssume with "[-]"); [done|]. iIntros "!>". rewrite bind_bind.
+    iApply (sim_gen_TGet with "[-]").
     iSplit. 1: done.
-    iIntros "!>".
-    rewrite bind_bind. iApply (sim_gen_TPut with "[Hs']"). 1: done.
+    iIntros "!>". rewrite bind_bind.
+    iApply (sim_gen_TPut with "[Hs]"). 1: done.
     iIntros "Hs". iIntros "!>".
-    iApply (sim_gen_TVis with "[-]"). iIntros (v') "Hs'".
+    iApply (sim_gen_TVis with "[-]"). iIntros (v'') "Hs'".
     iDestruct (mstate_var_agree with "Hs Hs'") as "<-".
     iIntros "!> /=".
     iIntros (??) "[% [% HΠ']]" => /=. simplify_eq.
     iApply "HC". simpl.
-    iSplit!. iFrame.
-    (* Here I need strong assumptions *)
-    iIntros (??) "[% [% H]]". subst.
-    iApply "HΠ". by iFrame.
-  Qed.
+    iSplit!.
+Qed.
 
-  Definition getc_fn_spec_priv (P: Z → iProp Σ) (es : list expr) (POST : (val → iProp Σ) → iProp Σ) : iProp Σ :=
-    ∃ v, ⌜es = []⌝ ∗ P v ∗
-    POST (λ v', (⌜v' = ValNum v⌝) ∗ P (v + 1))%I.
+  Definition getc_fn_spec (P : Z → iProp Σ) (es : list expr) (POST : (val → iProp Σ) → iProp Σ) : iProp Σ :=
+    ∃ v, P v ∗ ⌜es = []⌝ ∗ POST (λ ret, ⌜ret = v⌝ ∗ P (v + 1))%I.
 
-(* TODO : Maybe think about notation - more general for switch *)
-(* (WP (Spec.forever getc_spec_priv) @ Π' {{ e', sim_post Tgt () Π' e' }} -∗ σs ≈{spec_trans rec_event Z}≈>ₜ Π') *)
-
-  (* The actual P?: λ v. ∃ σs. spec_state v ∗ Q σs ∗ (TGT Spec.forever ... @ Π {}) -∗ σs ≈≈> Π *)
-  Lemma sim_getc_heap_priv Q fns Πr Πs :
+  Lemma sim_getc fns Π_l (P : Z → iProp Σ):
     rec_fn_auth fns -∗
     "getc" ↪ None -∗
-    Q (Spec.forever getc_spec_priv, 0) -∗ (* NOTE: Q needs to hold for the initial state of the module? - Am I okay with giving up Q? *)
-    □ switch_link_fixed Tgt Πr (spec_trans _ Z) Πs ({{ σr POST,
-      ∃ vs h' σs,
-      Q σs ∗
-      POST (ERCall "getc" vs h') σs ({{ _ Πs,
-        switch_link Tgt Πs ({{ σs' POST,
-          ∃ h'' v',
-            POST (ERReturn v' h'') _ σr ({{ _ Πr',
-              ⌜Πr' = Πr⌝ ∗ Q σs' }})}})}})}}) -∗
-    |==> ∃ P, P 0 ∗ □ rec_fn_spec_hoare Tgt Πr "getc" (getc_fn_spec_priv P).
+    switch Π_l ({{κ σ_l POST,
+      ∃ h v, ⌜κ = Some (Outgoing, ERCall "getc" [] h)⌝ ∗ P v ∗
+    POST Tgt _ (spec_trans _ Z) ({{σ_r Π_r,
+      ⌜σ_r = (getc_spec, v)⌝ ∗
+    switch Π_r ({{κ σ_r' POST,
+      ∃ e, ⌜κ = Some (Incoming, e)⌝ ∗
+    POST Tgt _ (spec_trans _ Z) ({{σ_r'' Π_r',
+      ⌜σ_r'' = σ_r'⌝ ∗ ⌜e = (ERCall "getc" [] h)⌝ ∗
+    switch Π_r' ({{κ σ_r''' POST,
+      ∃ h', ⌜κ = Some (Outgoing, ERReturn (ValNum v) h')⌝ ∗ ⌜σ_r''' = (getc_spec, (v + 1)%Z)⌝ ∗
+    POST Tgt _ _ ({{σ_l' Π_l',
+      ⌜σ_l' = σ_l⌝ ∗
+    switch Π_l' ({{κ σ_l'' POST,
+      ∃ e, ⌜κ = Some (Incoming, e)⌝ ∗
+    POST Tgt _ _ ({{σ_l''' Π_l',
+      ⌜σ_l'' = σ_l'''⌝ ∗ ⌜e = ERReturn v h'⌝ ∗ ⌜Π_l' = Π_l⌝ ∗ P (v + 1)
+      }})
+    }})}})}})}})}})}})}}) -∗
+    rec_fn_spec_hoare Tgt Π_l "getc" (getc_fn_spec P).
   Proof.
-    iIntros "#Hfns #Hf HQ #Hl /=".
-    iMod (mstate_var_alloc Z) as (γ) "Hγ".
-    iMod (mstate_var_split γ 0 with "[$]") as "[Hγ Hγ']".
-    pose (HS := SpecGS γ).
+    iIntros "#? ? Hs". iIntros (es Φ) "[% [HP [-> HΦ]]]".
+    iApply (sim_tgt_rec_Call_external with "[$]"). iIntros (???) "#??? !>".
+    iIntros (??) "[% [% HΠ]]". subst. iApply "Hs". iSplit!. iFrame. iIntros (??) "[-> Hs]".
 
-    (* have Π' : option (io_type * rec_ev) → m_state (spec_trans (io_type * rec_ev) Z) → iProp Σ. admit. *)
-    set (P := (λ (v : Z), (∃ σs, spec_state v ∗ Q σs ∗ (TGT (Spec.forever getc_spec_priv) @ Πs {{ e', sim_post Tgt () Πs e' }} -∗ σs ≈{spec_trans rec_event Z}≈>ₜ Πs))%I)).
-    iExists P.
-    iModIntro. iSplit.
-    - iExists (_, 0).
-      iFrame.
-      iIntros "?".
-      iApply (sim_gen_expr_intro with "[Hγ]") => /= //.
-    - iIntros "!> % % [% [-> [[% [Hs [HQ Hσs]]] HΦ]]]".
-      iApply (sim_tgt_rec_Call_external with "[$]").
-      iIntros (???) "#?Htoa Haa !>".
-      iIntros (? σr) "[% [% HΠr]]" => /=. subst.
-      iApply "Hl" => /=. iSplit!. iFrame. iSplit!.
-      iIntros (? Π'') "[-> [-> HΠs]]" => /=.
-      (* Here now I need to be talking about this specific Π - Should I pass this as parameter to the lemma? *)
-      (* assert (HProblem : Π'' = Π') by admit. subst. *)
-      iApply "Hσs". rewrite unfold_forever.
-      iApply sim_getc_spec_heap_priv.
-      iIntros (??) "[% [% [% [% Hσ]]]]" => /=.
-      iApply "HΠs" => /=. subst. iSplit!.
-      (* Π''' probably same as Πs, but I don't care *)
-      iIntros (? Πs') "[% [% HΠs']]". simplify_eq.
-      iApply "Hσ". iSplit!. iFrame.
-      iIntros (??) "[% [? HΠs]]" => /=.
-      iApply "HΠs'" => /=. subst. iSplit!.
-      iIntros (? HΠr') "[% HΠr']". subst.
-      iApply sim_tgt_rec_Waiting_raw.
-      iSplit. { iIntros. iModIntro. iApply "HΠr'". iSplit!. iIntros (??) "[% [% ?]]". simplify_eq. }
-      iIntros (???) "!>". iApply "HΠr'" => /=. iSplit!. iIntros (??) "[% [% [% HQ]]]". simplify_eq.
-      iApply "HΠr". iSplit!. iFrame.
-      iApply "HΦ". iSplit!. iFrame.
-      iIntros "Hspec".
-      iApply "HΠs". iSplit!.
+    iMod (mstate_var_alloc Z) as (γ) "?".
+    iMod (mstate_var_split γ v with "[$]") as "[Hγ Hγ']".
+    pose (Hspec := SpecGS γ).
+
+    iApply (sim_gen_expr_intro _ tt with "[Hγ]"); simpl; [done..|].
+    rewrite {2}/getc_spec.
+    rewrite unfold_forever bind_bind /TReceive bind_bind -/getc_spec.
+    iApply (sim_tgt_TExist with "[-]"). iIntros ([[??]?]) "!>".
+    rewrite bind_bind. setoid_rewrite bind_ret_l.
+    iApply (sim_gen_TVis with "[-]").
+    iIntros (v') "Hγ !>".
+    iIntros (??) "[% [% _]]".
+    subst.
+    iApply "Hs" => /=. iSplit!. iIntros (??) => /=.
+    iDestruct 1 as (??) "Hs". simplify_eq.
+
+    iApply (sim_gen_expr_intro _ tt with "[Hγ]"); simpl; [done..|]. rewrite bind_bind.
+    iApply (sim_tgt_TAssume with "[-]"); [done|]. iIntros "!>". rewrite bind_bind.
+    iApply (sim_tgt_TAssume with "[-]"); [done|]. iIntros "!>". rewrite bind_bind.
+    iApply (sim_gen_TGet with "[-]").
+    iSplit. 1: done.
+    iIntros "!>". rewrite bind_bind.
+    iApply (sim_gen_TPut with "[Hγ']"). 1: done.
+    iIntros "Hγ". iIntros "!>".
+    iApply (sim_gen_TVis with "[-]"). iIntros (v'') "Hγ'".
+    iDestruct (mstate_var_agree with "Hγ Hγ'") as "<-".
+    iIntros "!> /=".
+    iIntros (??) "[% [% _]]" => /=. simplify_eq.
+    iApply "Hs" => /=. iSplit!. iIntros (??) "[% Hs]". subst.
+
+    iApply sim_tgt_rec_Waiting_all_raw. iIntros (?) "!>".
+    iApply "Hs" => /=. iSplit!.
+    iIntros (??) "[% [% [% ?]]]" => /=. subst.
+
+    iApply "HΠ" => /=. iSplit!. iFrame. iApply "HΦ". by iFrame.
   Qed.
 
-End sim_spec.
+End sim_getc.
 
 (* ********************************************************************************************** *)
 (* Prove ⟦echo⟧_rec ⊕ ⟦getc⟧_spec ⪯ ⟦echo_getc⟧_spec *)
@@ -663,287 +173,161 @@ Section echo_getc.
 
   Context `{!dimsumGS Σ} `{!recGS Σ}.
 
-  (* TODO, experimental *)
-  Definition echo_getc_spec_body : spec rec_event Z unit :=
+  Definition echo_getc_spec_body : spec rec_event Z void :=
     v ← TGet;
     TPut (v + 1);;
     h ← TExist _;
     '(_, h') ← TCallRet "putc" [(ValNum v)] h;
     TAssume (h = h');;
-    TRet tt.
+    TUb.
 
   Definition echo_getc_spec : spec rec_event Z void :=
     '(f, vs, h) ← TReceive (λ '(f, vs, h), (Incoming, ERCall f vs h));
     TAssume (f = "echo");;
     TAssume (vs = []);;
-    Spec.forever echo_getc_spec_body.
+    echo_getc_spec_body.
 
-  (* Maybe it's more correct now *)
-  Lemma sim_echo_loop `{!specGS} Π P:
+  Definition echo_left_linkP γ_oe γ_q γ_r : Z → iProp Σ :=
+    (λ v, ∃ (q : list seq_product_case), γ_oe ⤳ @None rec_ev ∗ γ_q ⤳ q ∗ γ_r ⤳ (getc_spec, v))%I.
+
+  (* TODO REVIEW: Is this okay or not? *)
+  Lemma sim_echo Π v (P : Z → iProp Σ) :
     "echo" ↪ Some echo_rec -∗
-    □ rec_fn_spec_hoare Tgt Π "getc" (getc_fn_spec_priv P) -∗
-    rec_fn_spec_hoare Tgt Π "echo" ({{ es POST_m, ⌜es = []⌝ ∗
-      ∃ n, P n ∗
-      bi_loop ({{ LOOP v,
-        rec_fn_spec_hoare Tgt Π "putc" ({{ es POST,
-          ⌜es = [Val (ValNum v)]⌝ ∗
-        POST ({{ _,
-          LOOP (v + 1)
-        }})}})}}) n }}).
+    rec_fn_spec_hoare Tgt Π "getc" (getc_fn_spec P) -∗
+    rec_fn_spec_hoare Tgt Π "echo" (λ es POST, ⌜es = []⌝ ∗ P v ∗
+      rec_fn_spec_hoare Tgt Π "putc" (λ es POST1, P (v + 1) ∗ ⌜es = [Val v]⌝ ∗ POST1 (λ _, POST (λ ret, ⌜ret = 0⌝)))).
   Proof.
-    iIntros "#? #Hf". iApply rec_fn_spec_hoare_ctx.
-    (* NOTE What's up with the ordinal later stuff - recursion *)
-    iIntros "#?".
-    set BODY := (X in bi_loop X).
-    iApply ord_loeb. (*; [done|]*)
-    { iAssumption. }
-    iIntros "!> #IH".
-    iIntros (es Φ). iDestruct 1 as (->) "[% [HP HΦ]]".
+    iIntros "#? Hf".
+    iIntros (es Φ) => /=. iDestruct 1 as (->) "[HP HΦ]".
     iApply sim_tgt_rec_Call_internal. 2: { done. } { done. }
     iModIntro => /=.
-    iApply sim_tgt_rec_AllocA; [by econs|] => /=. iIntros (?) "?".
-    destruct ls as [|] => //=. iModIntro.
-    (* TODO: What's this `emp` thing here *)
-    iDestruct (bi_loop_unfold with "HΦ") as "HΦ". rewrite {2}/BODY => /=.
+    iApply sim_tgt_rec_AllocA; [by econs|] => /=. iIntros (?) "Hoof !>".
     iApply (sim_gen_expr_bind _ [LetECtx _ _] with "[-]") => /=.
-    iApply "Hf" => /=.
-    rewrite /getc_fn_spec_priv. iExists n.
-    iFrame. iSplit!. iIntros (?) "[% HP]".
-    iApply sim_tgt_rec_LetE => /=. iModIntro.
-    iApply (sim_gen_expr_bind _ [LetECtx _ _] with "[-]") => /=.
-    iApply "HΦ" => /=. simplify_eq. iSplit!.
-    iIntros (?) "HLOOP".
-    iApply sim_tgt_rec_LetE => /=. iModIntro.
-    iApply "IH" => /=. iSplit!. iFrame.
-  Qed.
 
-  (* TODO: This is probably fine for one call, but once I loop, how do I keep track of P *)
-  Lemma sim_echo `{!specGS} Π P n :
-    "echo" ↪ Some echo_rec -∗
-    P n -∗
-    □ rec_fn_spec_hoare Tgt Π "getc" (getc_fn_spec_priv P) -∗
-    rec_fn_spec_hoare Tgt Π "echo" ({{ es POST_m, ⌜es = []⌝ ∗
-      rec_fn_spec_hoare Tgt Π "putc" ({{ es POST_p,
-          ⌜es = [Val (ValNum n)]⌝ ∗
-          POST_p (λ _, POST_m (λ _, P (n + 1)))
-      }})}}).
-  Proof.
-    iIntros "#? HP #Hf".
-    iIntros (es Φ) => /=. iDestruct 1 as (->) "HΦ".
-    iApply sim_tgt_rec_Call_internal. 2: { done. } { done. }
-    iModIntro => /=.
-    iApply sim_tgt_rec_AllocA; [by econs|] => /=. iIntros (?) "_ !>".
-    iApply (sim_gen_expr_bind _ [LetECtx _ _] with "[-]") => /=.
-    iApply "Hf". iExists _. iSplit!. iFrame.
-    iDestruct 1 as (->) "HP".
+    iApply "Hf". iExists v. iFrame. iSplit!. iIntros (?) "[% ?]".
     iApply sim_tgt_rec_LetE. iIntros "!>" => /=.
     iApply (sim_gen_expr_bind _ [LetECtx _ _] with "[-]") => /=.
-    iApply "HΦ" => /=. by iFrame.
+    iApply "HΦ" => /=. iFrame. iSplit!.
+    iIntros "% HΦ".
+    iApply sim_tgt_rec_LetE. iIntros "!>" => /=.
+    iApply sim_gen_expr_stop. iSplit!.
+    iSplitL "Hoof".
+    { destruct ls; [by iApply big_sepL2_nil |done]. }
+    by iApply "HΦ".
   Qed.
 
-  (* TODO: Does a loop fix the Π *)
-
-  Lemma sim_echo_full_loop Π γσ_s (σ : m_state (spec_trans _ Z)) P :
+  Lemma sim_echo_full Π_t γs (σ_s : m_state (spec_trans _ Z)) γ_oe γ_q γ_r
+    (q : list seq_product_case) :
     "echo" ↪ Some echo_rec -∗
+    "getc" ↪ None -∗
     "putc" ↪ None -∗
-    □ rec_fn_spec_hoare Tgt Π "getc" (getc_fn_spec_priv P) -∗
-    γσ_s ⤳ σ -∗
-    ⌜σ.1 ≡ Spec.forever echo_getc_spec_body⌝ -∗
-    P σ.2 -∗ (* I require to own the token for the current module state *)
-    rec_fn_spec_hoare Tgt Π "echo" (λ es POST, ⌜es = []⌝ ∗
-      □ switch_external Π (λ κ σ POST,
-          ∃ vs h σ_s, ⌜κ = Some (Outgoing, ERCall "putc" vs h)⌝ ∗ γσ_s ⤳ σ_s ∗
-        POST (spec_trans _ Z) σ_s (λ _ Π',
-          ∃ e,
-        switch Π' (λ κ'' σ_s3 POST,
-          ⌜κ'' = Some (Incoming, e)⌝ ∗
-        POST Src _ _ (λ σ_s3' Π_s'',
-          ⌜σ_s3' = σ_s3⌝ ∗
-        switch Π_s'' (λ κ'' σ'' POST,
-          ∃ v h', ⌜e = ERReturn v h'⌝ ∗ ⌜κ'' = None⌝ ∗
-        POST Tgt _ _ (λ σ' Π',
-          ⌜σ' = σ⌝ ∗ γσ_s ⤳ σ'' ∗
-        switch Π' (λ κ σ POST,
-          ∃ e', ⌜κ = Some (Incoming, e')⌝ ∗
-        POST Tgt _ _ (λ σ' Π',
-          ⌜σ' = σ⌝ ∗ ⌜e = e'⌝ ∗ ⌜Π = Π'⌝)))))))) ∗
-      bi_loop ({{ LOOP v,
-          LOOP (v + 1)
-        }}) σ.2).
-      (* POST (λ _, ∃ v, γσ_s ⤳ (Spec.forever echo_getc_spec_body (T := void), v) ∗ P v)). *)
-  Proof. Admitted.
-(*     set (X := (switch_external _) _). *)
-(*     iIntros "#?#?#Hf Hσs % HP". iApply rec_fn_spec_hoare_ctx. iIntros "#?". *)
-
-(*     iApply ord_loeb. 1: done. *)
-(*     iIntros "!> #IH". *)
-
-(*     iIntros (??). iDestruct 1 as (?) "HLOOP". *)
-
-(*     iMod (mstate_var_alloc Z) as (γ) "H". *)
-(*     iMod (mstate_var_split γ σ.2 with "[$]") as "[Hγ Hγ']". *)
-(*     pose (Hspec := SpecGS γ). *)
-
-(*     iApply (sim_echo _ P _ with "[$] [HP //] [$]") => /=. subst. iSplit!. *)
-
-(*     (* NOTE: External Call to putc *) *)
-(*     iIntros (??). iDestruct 1 as (->) "HP". *)
-(*     iApply (sim_tgt_rec_Call_external); [done|]. *)
-(*     iIntros (???) "Hfns' Hh Ha !>". iIntros (??) "[-> [-> Hσ]]". *)
-(*     iApply "HX". iSplit!. iFrame. iSplit!. iIntros (??) "[-> HC]". *)
-(*     iApply (sim_gen_expr_intro _ tt with "[Hγ] [-]"); simpl; [done..|]. *)
-(*     rewrite {2}unfold_forever. rewrite bind_bind. *)
-(*     iApply sim_gen_TGet. iSplit. done. rewrite bind_bind. *)
-(*     iApply (sim_gen_TPut with "[$]"). iIntros "Hγ" => /=. rewrite bind_bind. *)
-(*     (* TODO: No idea if that makes sense *) *)
-(*     iApply (sim_src_TExist _). *)
-(*     rewrite /TCallRet. rewrite !bind_bind. (* That's annoying *) *)
-(*     iApply sim_gen_TVis. iIntros (?) "Hγ'". *)
-
-(*     iDestruct (mstate_var_agree with "Hγ Hγ'") as "<-". *)
-
-(*     iIntros (??) "[-> [-> _]]". *)
-(*     iApply "HC" => /=. iSplit!. iIntros (??) "[-> [% HC]]". *)
-(*     iApply (sim_gen_expr_intro _ tt with "[Hγ] [-]"); [simpl; done..|]. *)
-(*     rewrite bind_bind. iApply (sim_src_TExist e). rewrite bind_bind. *)
-
-(*     iApply sim_gen_TVis. iIntros (?) "Hγ". *)
-(*     iDestruct (mstate_var_agree with "Hγ Hγ'") as "->". *)
-(*     iIntros (??) "[-> [-> ?]]". *)
-(*     iApply "HC". iSplit!. *)
-(*     iIntros (??) "[% HC]". subst. *)
-
-(*     iApply (sim_gen_expr_intro _ tt with "[Hγ] [-]"); [simpl; done..|]. *)
-(*     destruct e. *)
-(*     { iApply sim_src_TUb. } *)
-(*     setoid_rewrite bind_ret_l. rewrite bind_bind. *)
-(*     iApply sim_src_TAssume. iIntros "->". *)
-(*     rewrite bind_ret_l. *)
-(*     iApply sim_gen_expr_None => /=. iIntros (???) "Hγ". *)
-(*     iDestruct (mstate_var_agree with "Hγ Hγ'") as "<-". *)
-(*     iIntros (??) "[% [% _]]" => /=. simplify_eq. *)
-
-(*     iApply "HC". iSplit!. iIntros (??) "[% [Hσs HC]]". subst. *)
-
-(*     iApply sim_tgt_rec_Waiting_raw. iSplit. *)
-(*     { iIntros (?????) "!>". iApply "HC". iSplit!. iIntros (??) "[% [% %]]". simplify_eq. } *)
-(*     iIntros (?? _) "!>". iApply "HC". *)
-(*     iSplit!. iIntros (??) "[-> [% <-]]". simplify_eq. *)
-(*     iApply "Hσ". iSplit!. *)
-(*     iFrame. *)
-(* Admitted. *)
-
-  (* NOTE: This does not seem horrible *)
-  Lemma sim_echo_full Π γσ_s (σ : m_state (spec_trans _ Z)) P :
-    "echo" ↪ Some echo_rec -∗
-    "putc" ↪ None -∗
-    □ rec_fn_spec_hoare Tgt Π "getc" (getc_fn_spec_priv P) -∗
-    γσ_s ⤳ σ -∗
-    ⌜σ.1 ≡ Spec.forever echo_getc_spec_body⌝ -∗
-    P σ.2 -∗ (* I require to own the token for the current module state *)
-    rec_fn_spec_hoare Tgt Π "echo" (λ es POST,
+    γs ⤳ σ_s -∗
+    γ_oe ⤳ @None rec_ev -∗
+    γ_q ⤳ q -∗
+    γ_r ⤳ (getc_spec, 0) -∗
+    rec_fn_spec_hoare Tgt Π_t "getc" (getc_fn_spec (echo_left_linkP γ_oe γ_q γ_r)) -∗
+    ⌜σ_s.1 ≡ echo_getc_spec_body⌝ -∗
+    ⌜σ_s.2 = 0⌝ -∗
+    rec_fn_spec_hoare Tgt Π_t "echo" ({{ es POST_e,
       ⌜es = []⌝ ∗
-      □ switch_external Π (λ κ σ POST,
-          ∃ vs h σ_s, ⌜κ = Some (Outgoing, ERCall "putc" vs h)⌝ ∗ γσ_s ⤳ σ_s ∗
-        POST (spec_trans _ Z) σ_s (λ _ Π',
-          ∃ e,
-        switch Π' (λ κ'' σ_s3 POST,
-          ⌜κ'' = Some (Incoming, e)⌝ ∗
-        POST Src _ _ (λ σ_s3' Π_s'',
-          ⌜σ_s3' = σ_s3⌝ ∗
-        switch Π_s'' (λ κ'' σ'' POST,
-          ∃ v h', ⌜e = ERReturn v h'⌝ ∗ ⌜κ'' = None⌝ ∗
-        POST Tgt _ _ (λ σ' Π',
-          ⌜σ' = σ⌝ ∗ γσ_s ⤳ σ'' ∗
-        switch Π' (λ κ σ POST,
-          ∃ e', ⌜κ = Some (Incoming, e')⌝ ∗
-        POST Tgt _ _ (λ σ' Π',
-          ⌜σ' = σ⌝ ∗ ⌜e = e'⌝ ∗ ⌜Π = Π'⌝)))))))) ∗
-      POST (λ _, ∃ v, γσ_s ⤳ (Spec.forever echo_getc_spec_body (T := void), v) ∗ P v)).
+      switch Π_t ({{ κ0 σ_t POST0,
+        ∃ vs h (σs : m_state (spec_trans rec_event Z)) (q : list seq_product_case) (r : m_state (spec_trans rec_event Z)),
+         γs ⤳ σs ∗ γ_oe ⤳ @None rec_ev ∗ γ_q ⤳ q ∗ γ_r ⤳ r ∗
+         ⌜κ0 = Some (Outgoing, ERCall "putc" vs h)⌝ ∗
+      POST0 Src _ (spec_trans _ Z) ({{ σ_s0 Π_s,
+        ⌜σ_s0 = σs⌝ ∗
+      switch Π_s ({{ κ1 σ_s1 POST1,
+        ⌜κ1 = κ0⌝ ∗
+      (* TODO: This is super counter-intuitive *)
+      POST1 Src _ (spec_trans _ Z) ({{ σ_s1' Π_s',
+        ⌜Π_s' = Π_s⌝ ∗ ⌜σ_s1 = σ_s1'⌝ ∗
+        ∃ e : rec_ev,
+      switch Π_s ({{ κ3 σ_s2 POST2,
+        ⌜κ3 = Some (Incoming, e)⌝ ∗
+      POST2 Src _ (spec_trans _ Z) ({{ σ_s2' Π_s',
+        ⌜Π_s' = Π_s⌝ ∗ ⌜σ_s2 = σ_s2'⌝ ∗
+      switch Π_s ({{ κ4 σ_s3 POST3,
+        ∃ v h', ⌜e = ERReturn v h'⌝ ∗ ⌜κ4 = None⌝ ∗
+      POST3 Tgt _ _ ({{ σ_t1 Π_t',
+        ⌜σ_t1 = σ_t⌝ ∗ γs ⤳ σ_s3 ∗ ⌜Π_t' = Π_t⌝ ∗
+      switch Π_t ({{ κ5 σ_t2 POST4,
+        ∃ e' : rec_ev, ⌜κ5 = Some (Incoming, e')⌝ ∗
+      POST4 Tgt rec_event rec_trans ({{ σ_t3 Π_t',
+        ⌜σ_t3 = σ_t2⌝ ∗ ⌜e = e'⌝ ∗ ⌜Π_t = Π_t'⌝ ∗ γ_oe ⤳ @None rec_ev ∗ γ_q ⤳ q ∗ γ_r ⤳ r
+      }})}})}})}})}})}})}})}})}})}}) ∗
+      POST_e (λ v, ⌜v = 0⌝)
+    }}).
   Proof.
-    set (X := (switch_external _) _).
-    iIntros "#?#?#Hf Hσs % HP". iIntros (??). iDestruct 1 as (?) "[#HX Hend]".
+    iIntros "#?#?#? Hγs Hγ_oe Hγ_q Hγ_r Hgetc %Hσ_s1 %Hσ_s2 %% [-> [Hs Hend]]" => /=.
 
-    iMod (mstate_var_alloc Z) as (γ) "H".
-    iMod (mstate_var_split γ σ.2 with "[$]") as "[Hγ Hγ']".
-    pose (Hspec := SpecGS γ).
+    iApply (sim_echo with "[//] Hgetc").
+    iSplit!. iFrame.
+    (* iIntros (??) "[? [-> HΦ']]".  *)
+    iIntros (??) "[[% [Hγ_oe [Hγ_q Hγ_r]]] [-> HΦ']]".
 
-    iApply (sim_echo _ P _ with "[$] [HP //] [$]") => /=. subst. iSplit!.
+    iApply (sim_tgt_rec_Call_external with "[$]").
+    iIntros (???) "#? ? ? !> %% [% [% HΠ]]" => /=. subst.
+    iApply "Hs" => /=. iSplit!. iFrame. iSplit!.
+    iIntros (? Πs) "[% Hs']" => /=. subst.
 
-    (* NOTE: External Call to putc *)
-    iIntros (??). iDestruct 1 as (->) "HP".
-    iApply (sim_tgt_rec_Call_external); [done|].
-    iIntros (???) "Hfns' Hh Ha !>". iIntros (??) "[-> [-> Hσ]]".
-    iApply "HX". iSplit!. iFrame. iSplit!. iIntros (??) "[-> HC]".
-    iApply (sim_gen_expr_intro _ tt with "[Hγ] [-]"); simpl; [done..|].
-    rewrite {2}unfold_forever. rewrite bind_bind.
-    iApply sim_gen_TGet. iSplit. done. rewrite bind_bind.
-    iApply (sim_gen_TPut with "[$]"). iIntros "Hγ" => /=. rewrite bind_bind.
-    (* TODO: No idea if that makes sense *)
-    iApply (sim_src_TExist _).
-    rewrite /TCallRet. rewrite !bind_bind. (* That's annoying *)
-    iApply sim_gen_TVis. iIntros (?) "Hγ'".
+    iMod (mstate_var_alloc Z) as (γs_s) "?".
+    iMod (mstate_var_split γs_s σ_s.2 with "[$]") as "[Hγs_s Hγs_s']".
+    pose (HSrcSpec := SpecGS γs_s).
 
-    iDestruct (mstate_var_agree with "Hγ Hγ'") as "<-".
+    iApply (sim_gen_expr_intro (Λ := spec_mod_lang (H := HSrcSpec) _ _ ) _ tt with "[Hγs_s] [-]"); [simpl; done..|].
 
-    iIntros (??) "[-> [-> _]]".
-    iApply "HC" => /=. iSplit!. iIntros (??) "[-> [% HC]]".
-    iApply (sim_gen_expr_intro _ tt with "[Hγ] [-]"); [simpl; done..|].
-    rewrite bind_bind. iApply (sim_src_TExist e). rewrite bind_bind.
+    iApply (sim_gen_TGet (H := HSrcSpec) with "[-]"). iSplit. 1: done.
+    iApply (sim_gen_TPut (H := HSrcSpec) with "[$]"). iIntros "Hγs_s".
+    iApply (sim_src_TExist (H := HSrcSpec)). rewrite bind_bind.
 
-    iApply sim_gen_TVis. iIntros (?) "Hγ".
-    iDestruct (mstate_var_agree with "Hγ Hγ'") as "->".
-    iIntros (??) "[-> [-> ?]]".
-    iApply "HC". iSplit!.
-    iIntros (??) "[% HC]". subst.
+    (* Here TCallRet *) (* TODO: What do the things I am throwing out allow me to do? *)
 
-    iApply (sim_gen_expr_intro _ tt with "[Hγ] [-]"); [simpl; done..|].
-    destruct e.
-    { iApply sim_src_TUb. }
-    setoid_rewrite bind_ret_l. rewrite bind_bind.
-    iApply sim_src_TAssume. iIntros "->".
-    rewrite bind_ret_l.
-    iApply sim_gen_expr_None => /=. iIntros (???) "Hγ".
-    iDestruct (mstate_var_agree with "Hγ Hγ'") as "<-".
+    iApply (sim_gen_TVis (H := HSrcSpec) with "[-]"). iIntros (?) "Hγs_s'".
+    iDestruct (mstate_var_agree with "Hγs_s Hγs_s'") as "<-".
     iIntros (??) "[% [% _]]" => /=. simplify_eq.
+    iApply "Hs'". iSplit!. by rewrite Hσ_s2.
+    iIntros (??) "[% [% [% Hs']]]" => /=. subst.
 
-    iApply "HC". iSplit!. iIntros (??) "[% [Hσs HC]]". subst.
-
-    iApply sim_tgt_rec_Waiting_raw. iSplit.
-    { iIntros (?????) "!>". iApply "HC". iSplit!. iIntros (??) "[% [% %]]". simplify_eq. }
-    iIntros (?? _) "!>". iApply "HC".
-    iSplit!. iIntros (??) "[-> [% <-]]". simplify_eq.
-    iApply "Hσ". iSplit!.
-    iFrame.
-Admitted.
+    iApply (sim_gen_expr_intro (Λ := spec_mod_lang (H := HSrcSpec) _ _ ) _ tt with "[Hγs_s] [-]"); [simpl; done..|].
+    rewrite bind_bind. iApply sim_src_TExist. rewrite bind_bind.
+    iApply (sim_gen_TVis (H := HSrcSpec) with "[-]"). iIntros (?) "Hγs_s".
+    iIntros (??) "[% [% _]]" => /=. subst.
+    iApply "Hs'" => /=. iSplit!.
+    iIntros (??) "[% [% Hs']]" => /=. subst.
+    iApply (sim_gen_expr_intro (Λ := spec_mod_lang (H := HSrcSpec) _ _ ) _ tt with "[Hγs_s] [-]"); [simpl; done..|].
+    destruct e. { iApply sim_src_TUb.  }
+    rewrite bind_ret_l. iApply sim_src_TAssume. iIntros "->". iApply sim_gen_expr_stop.
+    iIntros (?) "/= % Hγs_s". iApply sim_gen_stop.
+    iApply "Hs'" => /=. iSplit!.
+    iIntros (??)"[% [? [% Hs]]]". subst.
+    iApply sim_tgt_rec_Waiting_all_raw. iIntros (?) "!>".
+    iApply "Hs". iSplit!. iIntros (??) "[% [% [% ?]]]" => /=. subst.
+    iApply "HΠ" => /=. iSplit!. iFrame.
+    by iApply "HΦ'".
+  Qed.
 
   Let m_t := rec_link_trans {["echo"]} {["getc"]} rec_trans (spec_trans rec_event Z).
-  (* NOTE: Simulation statement: _ ⪯ (echo_getc_spec, v). The linked module (semantically)
-    refines the spec, i.e., for any sequence of silent (module internal) steps followed by a visible
-    event κ, the spec module can perform steps emitting κ. *)
+
   Lemma echo_getc_sim :
     rec_state_interp (rec_init echo_prog) None -∗
     (* TODO: Not exactly sure what the list is *)
-    (MLFRun None, [], rec_init echo_prog, (Spec.forever getc_spec_priv, 0)) ⪯{m_t,
+    (MLFRun None, [], rec_init echo_prog, (getc_spec, 0)) ⪯{m_t,
       spec_trans rec_event Z} (echo_getc_spec, 0).
   Proof.
     iIntros "[#Hfns [Hh Ha]] /=".
 
-    (* (* REVIEW: Am I saying here that I have r/w over the modules, and when I step through one *)
-    (*    I ensure I cannot change the other by splitting the var? *) *)
-    iMod (mstate_var_alloc (m_state (spec_trans rec_event Z))) as (γσ_s) "Hγσ_s".
-    iMod (mstate_var_alloc (m_state m_t)) as (γσ_t) "Hγσ_t".
+    iMod (mstate_var_alloc (m_state (spec_trans rec_event Z))) as (γs) "Hγs".
+    (* Entire Target Module *)
+    iMod (mstate_var_alloc (m_state m_t)) as (γt) "Hγt".
+    (* Event *)
     iMod (mstate_var_alloc (option rec_event)) as (γκ) "Hγκ".
 
-    iMod (mstate_var_alloc Z) as (γs_s) "Hγs_t".
+    (* Source's spec state *)
+    iMod (mstate_var_alloc Z) as (γs_s) "?".
     iMod (mstate_var_split γs_s 0 with "[$]") as "[Hγs_s Hγs_s']".
     pose (HSrcSpec := SpecGS γs_s).
 
-    (* iMod (mstate_var_alloc Z) as (γs_t) "?". *)
-    (* iMod (mstate_var_split γs_t v with "[$]") as "[Hγs_t Hγs_t']". *)
-    (* pose (HTgtSpec := SpecGS γs_t). *)
-
-    iApply (sim_tgt_constP_intro γσ_t γσ_s γκ with "Hγσ_t Hγσ_s Hγκ [-]"). iIntros "Hγσ_s".
+    iApply (sim_tgt_constP_intro γt γs γκ with "Hγt Hγs Hγκ [-]"). iIntros "Hγs".
     (* NOTE: I am fixing here the state of the spec in the source *)
     iApply (sim_tgt_link_None with "[-]"). iIntros "!>" (??????).
     (* NOTE: Case splitting on the linking case, which can only be a call because of the empty list  *)
@@ -951,151 +335,141 @@ Admitted.
     destruct!/=. case_match; destruct!/=.
 
     (* NOTE: Changing to source module *)
-    iApply (sim_tgt_constP_elim γσ_t γσ_s γκ with "[Hγσ_s] [-]"); [done..|].
-    iIntros "Hγσ_s Hγσ_t Hγκ".
+    iApply (sim_tgt_constP_elim γt γs γκ with "[Hγs] [-]"); [done..|].
+    iIntros "Hγs Hγt Hγκ".
     (* NOTE: Now, going into module local reasoning - Giving up one half of the state *)
     iApply (sim_gen_expr_intro (Λ := spec_mod_lang (H := HSrcSpec) _ _ ) _ tt with "[Hγs_s] [-]"); [simpl; done..|].
     iEval (unfold echo_getc_spec). rewrite /TReceive bind_bind.
     iApply (sim_src_TExist (H := HSrcSpec) (_, _, _)).
     rewrite bind_bind. setoid_rewrite bind_ret_l.
-    iApply (sim_gen_TVis (H := HSrcSpec)). iIntros (v') "Hγs_s". rewrite /spec_state /spec_state_name.
-    (* TODO: switch_id here *)
-    (* FIXME, discarding something here *)
-    iIntros (??) "[-> [-> _]]".
-    iApply (sim_src_constP_next with "[Hγσ_t] [Hγκ] [Hγσ_s] [%] [-]"); [done..|].
+    iApply (sim_gen_TVis (H := HSrcSpec)). iIntros "% Hγs_s %% [-> [-> _ ]]".
+
+    iApply (sim_src_constP_next with "[Hγt] [Hγκ] [Hγs] [%] [-]"); [done..|].
     (* NOTE: I unify here *)
     iDestruct (mstate_var_agree with "Hγs_s Hγs_s'") as "->".
 
-    iIntros "Hγσ_s". iApply sim_gen_stop.
-    (* NOTE: I am here going right back into the src module, to get the function name from the assume *)
-    iApply (sim_tgt_constP_elim γσ_t γσ_s γκ with "[Hγσ_s] [-]"); [done..|].
-    iIntros "Hγσ_s Hγσ_t Hγκ".
-    (* NOTE - Here I give up my state again *)
+    iIntros "Hγs". iApply sim_gen_stop.
+    iApply (sim_tgt_constP_elim γt γs γκ with "[Hγs] [-]"); [done..|].
+    iIntros "Hγs Hγt Hγκ".
+
     iApply (sim_gen_expr_intro (Λ := spec_mod_lang (H := HSrcSpec) _ _ ) _ tt with "[Hγs_s] [-]"); [simpl; done..|].
     iApply (sim_src_TAssume (H := HSrcSpec)). iIntros (?).
     iApply (sim_src_TAssume (H := HSrcSpec)). iIntros (?). simplify_eq.
     iApply sim_gen_expr_None => /=. iIntros (? [] ?) "Hγs_s".
-    (* NOTE: Got it back again - and it's linked to the state *)
+
+    (* iDestruct (mstate_var_merge with "Hγs_s Hγs_s'") as "[<- Hγs_s]". *)
+
     iIntros (??) "[-> [-> _]]".
     (* NOTE: The source module here is in a good spot for induction. In target the recursion is on the echo, but
        this is an internal call? So where do I start the recursion? *)
-    (* iDestruct (mstate_var_agree with "Hγs_s Hγs_s'") as "->". *)
 
     (* NOTE: Changing into target *)
     rewrite bool_decide_true; [|done].
-    iApply (sim_src_constP_next with "[Hγσ_t] [Hγκ] [Hγσ_s] [%] [-]"); [done..|].
-    iIntros "Hγσ_s".
-    iApply (sim_tgt_link_left_recv with "[-]").
-    (* NOTE: Again, this waiting_raw, which has the extra case for returning events *)
+    iApply (sim_src_constP_next with "[Hγt] [Hγκ] [Hγs] [%] [-]"); [done..|].
+    iIntros "Hγs".
+    iApply (sim_tgt_link_recv_left with "[-]").
     iApply (sim_tgt_rec_Waiting_raw _ []).
     iSplit; [|by iIntros].
     iIntros (???? Hin) "!> %". simplify_map_eq.
 
-    (* (* TODO: Here switching *) *)
-    iApply (sim_tgt_link_left with "[-]").
+    (* Target's spec module (Right linking case - getc) *)
+    iMod (mstate_var_alloc (m_state (spec_trans rec_event Z))) as (γt_r) "Hγt_r".
+
+    (* TODO: "queue" for linking?  *)
+    iMod (mstate_var_alloc (list seq_product_case)) as (γt_q) "Hγt_q".
+
+    (* (* Linking event to pass around *) *)
+    iMod (mstate_var_alloc (option rec_ev)) as (γt_oe) "Hγt_oe".
+
+    iApply (sim_tgt_link_left_const_run γt_q γt_r γt_oe with "[$] [$] [$] [-]").
+    iIntros "Hγt_q Hγt_r Hγt_oe".
+
     iMod (rec_mapsto_alloc_big (h_heap h) with "Hh") as "[Hh _]". { apply map_disjoint_empty_r. }
 
     iApply (sim_gen_expr_intro _ [] with "[Hh Ha]"). { done. }
     { rewrite /= /rec_state_interp dom_empty_L right_id_L /=. iFrame "#∗". by iApply rec_alloc_fake. }
 
-    (* (* TODO: This is dangerous now, as it contains the state *) *)
-    set (Π := link_tgt_leftP _ _ _ _).
+    set (Π_s := sim_src_constP γκ γt (EV := rec_event) (m_t := m_t) (m_s := spec_trans rec_event Z)).
+    set (Π_t := tgt_link_left_constP _ _ _ _ _).
 
     iApply (sim_gen_expr_bind _ [ReturnExtCtx _] with "[-]") => /=.
 
-    have Πs : option (io_type * rec_ev) → m_state (spec_trans (io_type * rec_ev) Z) → iProp Σ.
-    (* exact (@sim_tgt_constP Σ rec_event dimsumGS0 m_t (spec_trans rec_event Z) γσ_t γσ_s γκ).  *)
-    admit.
-    iAssert (□ switch_link_fixed Tgt Π (spec_trans (io_event rec_ev) Z) Πs ({{ σr POST,
-            ∃ (vs : list val) (h' : heap_state) (σs : spec rec_event Z void * Z), True ∗
-              POST (ERCall "getc" vs h') σs ({{ _ Πs,
-                switch_link Tgt Πs ({{ _ POST0,
-                  ∃ (h'' : heap_state) (v' : val),
-                    POST0 (ERReturn v' h'') rec_mod_lang σr ({{ _ Πr', ⌜Πr' = Π⌝ ∗ True}})}})}})}}))%I as "H2".
-    { iIntros "!> % %" => /=. iDestruct 1 as (???) "[_ [% HC]]". subst.
+    iDestruct (mstate_var_merge with "Hγs_s Hγs_s'") as "[% Hγs_s]".
+
+    rewrite /echo_prog in Hin. simplify_map_eq.
+
+    iApply (sim_echo_full with "[] [] [] Hγs Hγt_oe Hγt_q Hγt_r [] [//] [//]"). 1-3: by iApply (rec_fn_intro with "[$]") => /=.
+    {
+      iApply (sim_getc with "[//]"). by iApply (rec_fn_intro with "[$]").
+      iIntros (??).
+      (* iDestruct 1 as (?? ->) "[[% [Hγt_oe [Hγt_q Hγt_r]]] HC]" => /=. *)
+      iDestruct 1 as (?? ->) "[[% [Hγt_oe [Hγt_q Hγt_r]]] HC]" => /=.
+
+      iIntros "%%% Hγt_q' Hγt_r' Hγt_oe'".
+
+      iDestruct (mstate_var_merge with "Hγt_r Hγt_r'") as "[<- Hγt_r]".
+      iDestruct (mstate_var_merge with "Hγt_oe Hγt_oe'") as "[<- Hγt_oe]".
+      iDestruct (mstate_var_merge with "Hγt_q Hγt_q'") as "[<- Hγt_q]".
       iIntros (??????). destruct!/=. rewrite bool_decide_false //. rewrite bool_decide_true //.
-      iApply (sim_tgt_link_right_recv with "[-]").
-      iApply "HC". iSplit. admit.
-      iSplit. simpl. admit.
-      iIntros (??) "[% [-> HC]] %" => /=. simplify_eq.
-      iApply (sim_tgt_link_right with "[-]"). iApply "HC". iSplit!.
-      iIntros (??) => /=. iDestruct 1 as (?? ->) "HC".
+      iApply (sim_tgt_link_recv_right with "[-]"). iApply "HC". iSplit!. iIntros (??). iDestruct 1 as (? ->) "HC" => /=.
+      iIntros (?). simplify_eq.
+      iApply (sim_tgt_link_run_right with "[-]"). iApply "HC". iSplit!.
+      iIntros (??). iDestruct 1 as (??) "[% HC]" => /=. simplify_eq.
       iIntros (??????). destruct!/=.
-      iApply (sim_tgt_link_left_recv with "[-]").
+      iApply (sim_tgt_link_left_const_recv γt_q γt_r γt_oe with "[$] [Hγt_r] [$] [-]"). 1: done.
+      iIntros "Hγt_q Hγt_r Hγt_oe".
       iApply "HC". iSplit!.
-      iIntros (??) => /=. iDestruct 1 as (?->) "HC". iIntros. simplify_eq.
-      iApply (sim_tgt_link_left with "[-]"). iApply "HC".
-      iSplit!. admit. }
-
-    iAssert ("getc" ↪ None)%I as "H1". { by iApply (rec_fn_intro with "[$]"). }
-    iPoseProof (sim_getc_heap_priv (λ _, True)%I _ _ _ with "Hfns H1") as "H".
-
-    iAssert ("getc" ↪ None)%I as "H".   -∗
-    Q (Spec.forever getc_spec_priv, 0) -∗ (* NOTE: Q needs to hold for the initial state of the module? - Am I okay with giving up Q? *)
-    □ switch_link_fixed Tgt Πr (spec_trans _ Z) Πs ({{ σr POST,
-      ∃ vs h' σs,
-      Q σs ∗
-      POST (ERCall "getc" vs h') σs ({{ _ Πs,
-        switch_link Tgt Πs ({{ σs' POST,
-          ∃ h'' v',
-            POST (ERReturn v' h'') _ σr ({{ _ Πr',
-              ⌜Πr' = Πr⌝ ∗ Q σs' }})}})}})}}) -∗
-    |==> ∃ P, P 0 ∗ □ rec_fn_spec_hoare Tgt Πr "getc" (getc_fn_spec_priv P).
-
-    (* (* NOTE: Here I am using my state *) *)
-    iApply (sim_echo_full with "[] [] [] [Hγσ_s //] [//] [Hγs_s //]"). 1-2: by iApply (rec_fn_intro with "[$]").
-    { (* NOTE: And immediately give it up *)
-      iApply (sim_getc_heap_priv with "[] [] [Hγs_t]").
-      1: done. 1: by iApply (rec_fn_intro with "[$]"). 1: done.
-      iIntros (??) => /=. iDestruct 1 as (??->) "HC". iIntros => /=.
-      iIntros (??????). destruct!/=. rewrite bool_decide_false // bool_decide_true //.
-      iApply (sim_tgt_link_right_recv with "[-]") => /=. iApply "HC". iSplit!.
       iIntros (??). iDestruct 1 as (? ->) "HC" => /=.
-      iIntros (?). simplify_eq.
-      iApply (sim_tgt_link_right with "[-]"). iApply "HC". iSplit!.
-      iIntros (??) => /=. iDestruct 1 as (?? ->) "[Hγs_t [-> HC]]" => /=.
-      iIntros (??????). destruct!/=.
-      iApply (sim_tgt_link_left_recv with "[-]"). iApply "HC". iSplit!.
-      iIntros (??). iDestruct 1 as (? ->) "HC" => /=.
-      iIntros (?). simplify_eq.
-      iApply (sim_tgt_link_left with "[-]"). iApply "HC".
+      iIntros "%%% Hγt_q' Hγt_r' Hγt_oe'".
+      iDestruct (mstate_var_merge with "Hγt_r Hγt_r'") as "[<- Hγt_r]".
+      iDestruct (mstate_var_merge with "Hγt_oe Hγt_oe'") as "[<- Hγt_oe]".
+      iDestruct (mstate_var_merge with "Hγt_q Hγt_q'") as "[<- Hγt_q]". iIntros (?). simplify_eq.
+      iApply (sim_tgt_link_left_const_run γt_q γt_r γt_oe with "[$] [Hγt_r] [$] [-]"). 1: done.
+      iIntros "Hγt_q Hγt_r Hγt_oe".
+      iApply ("HC" with "[-]"). iSplit!. iFrame.
+    }
+    iSplit!.
+    iSplitL.
+    - iIntros (??) "[% [% [% [% [% [Hγs [Hγt_oe [Hγt_q [Hγt_r [% HC]]]]]]]]]]" => /=.
+      subst. iIntros (???) "Hγt_q' Hγt_r' Hγt_oe'".
 
-      iDestruct (mstate_var_agree with "Hγs_t Hγs_t'") as "->".
-      iSplit!.
-    (* } *)
-    (* iSplit!. *)
-    (* (* TODO: This is just copied over... *) *)
-    (* - iIntros "!>" (??). iDestruct 1 as (??? ->) "[Hγσ_s HC]" => /=. *)
-    (*   iIntros  (??????). destruct!/=. rewrite !bool_decide_false //. *)
-    (*   iApply (sim_tgt_constP_elim γσ_t γσ_s γκ with "[Hγσ_s] [-]"); [done..|]. *)
-    (*   iIntros "Hγσ_s Hγσ_t Hγκ". *)
-    (*   iApply "HC". iSplit!. iIntros (??). iDestruct 1 as (->) "HC". *)
-    (*   iApply (sim_src_constP_next with "[Hγσ_t] [Hγκ] [Hγσ_s] [%] [-]"); [done..|]. *)
-    (*   iIntros "Hγσ_s". *)
-    (*   iApply (sim_tgt_link_None with "[-]"). iIntros "!>" (??????). destruct!/=. *)
-    (*   iApply (sim_tgt_constP_elim γσ_t γσ_s γκ with "[Hγσ_s] [-]"); [done..|]. *)
-    (*   iIntros "Hγσ_s Hγσ_t Hγκ". *)
-    (*   iApply "HC". iSplit!. iIntros (??) "[% HC]". simplify_eq. *)
-    (*   iApply (sim_src_constP_next with "[Hγσ_t] [Hγκ] [Hγσ_s] [%] [-]"); [done..|]. *)
-    (*   iIntros "Hγσ_s". iApply sim_gen_stop. *)
-    (*   iApply (sim_tgt_constP_elim γσ_t γσ_s γκ with "[Hγσ_s] [-]"); [done..|]. *)
-    (*   iIntros "Hγσ_s Hγσ_t Hγκ". *)
-    (*   iApply "HC". iSplit!. iIntros (??). iDestruct 1 as (?? -> ->) "HC". *)
-    (*   iApply (sim_src_constP_next with "[Hγσ_t] [Hγκ] [Hγσ_s] [%] [-]"); [done..|]. *)
-    (*   iIntros "Hγσ_s". destruct!/=. *)
-    (*   iApply (sim_tgt_link_left_recv with "[-]"). *)
-    (*   iApply ("HC" with "[-]"). iFrame. iSplit!. *)
-    (*   iIntros (??). iDestruct 1 as (? ->) "HC". *)
-    (*   iIntros (?). simplify_eq. *)
-    (*   iApply (sim_tgt_link_left with "[-]"). *)
-    (*   iApply "HC". iSplit!. *)
-    (* - iIntros (?) "[% [Hγσ_s Hs]]". iApply sim_tgt_rec_ReturnExt. *)
-    (*   iIntros (???) "Hfns''' Hh Ha !>". *)
-    (*   iIntros (??) "[-> [-> _]]" => /=. iIntros (??????). destruct!/=. *)
-    (*   iApply (sim_tgt_constP_elim γσ_t γσ_s γκ with "[Hγσ_s] [-]"); [done..|]. *)
-    (*   iIntros "Hγσ_s Hγσ_t Hγκ". *)
-    (*   iApply "Hs". *)
-    (* Qed. *)
-  Admitted.
+      iDestruct (mstate_var_merge with "Hγt_r Hγt_r'") as "[<- Hγt_r]".
+      iDestruct (mstate_var_merge with "Hγt_oe Hγt_oe'") as "[<- Hγt_oe]".
+      iDestruct (mstate_var_merge with "Hγt_q Hγt_q'") as "[<- Hγt_q]".
+      iIntros (??????). destruct!/=. rewrite bool_decide_false //.
+
+      iApply (sim_tgt_constP_elim γt γs γκ with "[Hγs] [-]"); [done..|].
+      iIntros "Hγs Hγt Hγκ".
+      iApply "HC". iSplit!. iIntros (??). iDestruct 1 as (->) "HC".
+      iApply (sim_src_constP_next with "[Hγt] [Hγκ] [Hγs] [%] [-]"); [done..|].
+      iIntros "Hγs".
+      iApply (sim_tgt_link_None with "[-]"). iIntros "!>" (??????). destruct!/=.
+      iApply (sim_tgt_constP_elim γt γs γκ with "[Hγs] [-]"); [done..|].
+      iIntros "Hγs Hγt Hγκ".
+      iApply "HC". iSplit!. iIntros (??) "[% HC]". simplify_eq.
+      iApply (sim_src_constP_next with "[Hγt] [Hγκ] [Hγs] [%] [-]"); [done..|].
+      iIntros "Hγs". iApply sim_gen_stop.
+      iApply (sim_tgt_constP_elim γt γs γκ with "[Hγs] [-]"); [done..|].
+      iIntros "Hγs Hγt Hγκ".
+      iApply "HC". iSplit!. iIntros (??). iDestruct 1 as (?? -> ->) "HC".
+      iApply (sim_src_constP_next with "[Hγt] [Hγκ] [Hγs] [%] [-]"); [done..|].
+      iIntros "Hγs". destruct!/=.
+      iApply (sim_tgt_link_left_const_recv γt_q γt_r γt_oe with "[$] [Hγt_r] [$] [-]"). 1: done.
+      iIntros "Hγt_q Hγt_r Hγt_oe".
+      iApply ("HC" with "[-]"). iFrame. iSplit!.
+      iIntros (??). iDestruct 1 as (? ->) "HC".
+      iIntros (???) "Hγt_q' Hγt_r' Hγt_oe'".
+
+      iDestruct (mstate_var_merge with "Hγt_r Hγt_r'") as "[<- Hγt_r]".
+      iDestruct (mstate_var_merge with "Hγt_oe Hγt_oe'") as "[<- Hγt_oe]".
+      iDestruct (mstate_var_merge with "Hγt_q Hγt_q'") as "[<- Hγt_q]".
+      iIntros (?). simplify_eq.
+
+      iApply (sim_tgt_link_left_const_run γt_q γt_r γt_oe with "[$] [Hγt_r] [$] [-]"). 1: done.
+      iIntros "???".
+
+      iApply "HC". iSplit!. iFrame.
+    - admit.
+    Admitted.
 
 End echo_getc.
